Finish the proof.
git-svn-id: svn+ssh://scm.gforge.inria.fr/svn/coqcert/trunk/cic-model@125 7b0040dd-6dd6-45fd-888d-7922243e4794

Embedding.v
@@ -1,4 +1,4 @@
-Require Import TheoryInTerm.
+Require Import CCTnat.
 
 Import BuildModel.
 Import CCM.
@@ -50,7 +50,7 @@ red; intros. simpl.
 apply vcons_add_var; [apply H | apply H0]; trivial.
 Qed.
 
-Lemma embedding : forall env1 env2 s t A, A <> None ->
+Lemma embedding' : forall env1 env2 s t A, A <> None ->
   typ_esub env1 s env2 ->
   typ env2 t A -> 
   typ env1 (app_esub s t) (app_esub s A).
@@ -68,4 +68,125 @@ replace (fun k : nat => esub_conv s x0 k) with (esub_conv s x0); trivial.
 replace (esub_conv s (fun k : nat => y0 k)) with (esub_conv s y0); trivial.
 apply ZFind_basic.EQ_morph; [|rewrite H|rewrite H]; reflexivity.
 Qed.
+
+Definition eq_fosub n' e s s' := forall n, n < n' ->
+  eq_typ e (app_esub s (Ref n)) (app_esub s' (Ref n)) /\
+  typ e (app_esub s (Ref n)) T /\ typ e (app_esub s' (Ref n)) T.
+
+Fixpoint max_var_rec (t:foterm) max_v :=
+  match t with
+    | Var n => Peano.max max_v n
+    | Cst_0 => max_v
+    | Cst_1 => max_v
+    | Df_Add m n => Peano.max (max_var_rec m max_v) (max_var_rec n max_v) 
+  end.
+
+Definition max_var t := max_var_rec t 0.
+
+Fixpoint const_env n := 
+  match n with
+    | 0 => T :: nil
+    | S m => T :: (const_env m)
+  end.
+
+Lemma succ_max_distr : forall n m, S (Peano.max n m) = Peano.max (S n) (S m).
+induction n; destruct m; simpl; reflexivity.
+Qed.
+
+Lemma max_split1 : forall x y z, z < x -> z < Peano.max x y.
+induction x; simpl; intros.
+ apply False_ind; omega.
+
+ destruct y; trivial.
+  destruct z; try omega.
+   assert (z < x) by omega. specialize IHx with (1:=H0) (y:=y). omega.
+Qed.
+
+Lemma max_split2 : forall x y z, z < y -> z < Peano.max x y.
+induction x; simpl; intros; trivial.
+ destruct y; trivial.
+  apply False_ind; omega.
+ 
+  destruct z; try omega.
+   assert (z < y) by omega. specialize IHx with (1:=H0). omega.
+Qed.
+
+Lemma max_comb : forall x y z, z < Peano.max x y -> z < x \/ z < y.
+induction x; simpl; intros.
+ right; trivial.
+
+ destruct y.
+  left; trivial.
+
+  destruct z.
+   left; omega.
+
+   assert (z < Peano.max x y) by omega.
+   specialize IHx with (1:=H0). destruct IHx; [left | right]; omega.
+Qed.
+
+Lemma const_env_spec : forall m n t, 
+  nth_error (const_env n) m = value t ->
+  m <= n /\ t = T.
+induction m; destruct n; simpl; intros.
+ injection H; intros; split; [|subst t]; trivial.
+
+ injection H; intros; split; [omega |subst t]; trivial.
+
+ destruct m; simpl in H; discriminate.
+
+ specialize IHm with (1:=H). destruct IHm.
+ split; [omega | trivial].
+Qed.
+
+Lemma impl_and_split : forall A B C, (A -> B /\ C) -> ((A -> B)/\(A->C)).
+split; intros H1; specialize H with (1:=H1); destruct H; trivial.
+Qed.
+
+Lemma embedding : forall e t1 t2 s s',
+  eq_typ (const_env (Peano.max (max_var t1) (max_var t2)))
+  (int_fotrm t1) (int_fotrm t2) ->
+  eq_fosub (S (Peano.max (max_var t1) (max_var t2))) e s s' ->
+  eq_typ e (app_esub s (int_fotrm t1)) (app_esub s' (int_fotrm t2)).
+do 2 red; simpl; intros.
+do 2 red in H; simpl.
+unfold eq_fosub in H0.
+assert (val_ok (const_env (Peano.max (max_var t1) (max_var t2))) (esub_conv s i)).
+ unfold val_ok. do 2 red; intros. apply const_env_spec in H2.
+ destruct H2; subst T; simpl.
+ assert (n < S (Peano.max (max_var t1) (max_var t2))) by omega.
+ specialize H0 with (1:=H3); destruct H0 as (Heqtyp, (Htyps, Htyps')).
+ do 2 red in Htyps; simpl in Htyps; specialize Htyps with (1:=H1). apply Htyps.
+
+specialize H with (1:=H2). rewrite H.
+replace (fun k : nat => i k) with i; trivial. clear H H2.
+
+induction t2; simpl; try reflexivity.
+ specialize H0 with (n0:=n). destruct H0.
+  rewrite succ_max_distr. apply max_split2. unfold max_var; simpl; omega.
+  do 2 red in H; simpl in H; apply H; trivial.
+
+ apply NATREC_morph.
+  apply IHt2_1. intros. apply H0.
+  rewrite succ_max_distr. rewrite succ_max_distr in H. 
+  apply max_comb in H. destruct H.
+   apply max_split1; trivial.
+
+   apply max_split2. unfold max_var; simpl.
+   rewrite succ_max_distr. apply max_split1. trivial.
+
+  do 2 red; intros. rewrite H2; reflexivity.
+
+  apply IHt2_2. intros. apply H0.
+  rewrite succ_max_distr. rewrite succ_max_distr in H. 
+  apply max_comb in H. destruct H.
+   apply max_split1; trivial.
+
+   apply max_split2. unfold max_var; simpl.
+   rewrite succ_max_distr. apply max_split2. trivial.
+Qed.
+
+
+
+
   
